GoCFG.v
@@ -18,6 +18,7 @@ Require Import Coq.Lists.List.
 From Stdlib Require Import Lia.
 From Stdlib Require Import Arith.
 From Fido Require Import GoRuntimeTypes.
+From Fido Require Import GoEffects.
 From Fido Require Import builtins.
 
 Inductive Next : Type :=
