GoSem.v
@@ -23,6 +23,7 @@
 From Fido Require Import GoAst GoTypes GoSafe cmd preamble.   (* [preamble] re-exports [builtins]: [GoAny]/[anyt]/[intwrap]/[World]/[w_log]/[Outcome]/[ORet] *)
 From Fido Require Import GoNumeric.
 From Fido Require Import GoRuntimeTypes.
+From Fido Require Import GoEffects.
 From Fido Require Export GoSemCore.
 From Fido Require Export GoSemDenote.
 From Stdlib Require Import String List Bool ZArith Lia.
